coq/theories/imp2asm/ImpToASMCodegenProofs.v
@@ -67,33 +67,37 @@ Definition has_stack (t : ASMSemantics.state) (xs : list word_or_ret) : Prop :=
     t.(regs) RAX = Some w /\
     t.(stack) = ws.
 
-Definition v_arr_inv (asmm: word64 -> option (option word64))
-  (block: list (option Value)) (vasm: option word64): Prop :=
-  forall i v,
-    List.nth_error block i = Some v ->
-    exists w,
-      v = Some (ImpSyntax.Word w) /\
-      match vasm with
-      | Some base =>
-          asmm (word.add base (word.of_Z (Z.of_nat i * 8))) = Some (Some w)
-      | None => False
-      end.
+Definition opt_rel {A B} (P: A -> B -> Prop) (oa: option A) (ob: option B): Prop :=
+  match oa, ob with
+  | None, None => True
+  | Some a, Some b => P a b
+  | _, _ => False
+  end.
 
-(* Constrains v to valid ranges and equates it with w in the context of ASM state t. *)
-Definition v_inv (asmm: word64 -> option (option word64)) (impm: list (list (option Value)))
+Definition v_inv (pmap: nat -> option (word64 * nat))
   (v: Value) (w: word64): Prop :=
   match v with
-  | ImpSyntax.Word v => word.ltu v (word.of_Z (2 ^ 63)) = true /\ w = v
-  | Pointer p =>
-    match List.nth_error impm p, asmm w with
-    | Some block, Some asmv =>
-      v_arr_inv asmm block asmv
-    | _, _ => False
-    end
+  | ImpSyntax.Word v => w = v
+  | Pointer p => exists length,
+    pmap p = Some (w, length)
   end.
+
+Definition mem_inv (pmap: nat -> option (word64 * nat))
+  (asmm: word64 -> option (option word64))
+  (impm: list (list (option Value))): Prop :=
+  forall p v,
+    List.nth_error impm p = Some v ->
+    exists base,
+      pmap p = Some (base, List.length v) /\
+      forall off xopt,
+        List.nth_error v off = Some xopt ->
+        exists yopt,
+          asmm (word.add base (word.of_Z (Z.of_nat (off * 8)))) = Some yopt /\
+          opt_rel (v_inv pmap) xopt yopt.
 
 (* Checks that environment variables map to valid locations and values on the stack in the ASM state. *)
 Definition env_ok (env : IEnv.env) (vs : list (option nat)) (curr : list word_or_ret)
+  (pmap: nat -> option (word64 * nat))
   (asmm : word64 -> option (option word64))
   (impm: list (list (option Value))): Prop :=
   List.length vs = List.length curr /\
@@ -102,12 +106,15 @@ Definition env_ok (env : IEnv.env) (vs : list (option nat)) (curr : list word_or
     index_of n 0 vs < List.length curr /\
     exists w,
       nth_error curr (index_of n 0 vs) = Some (Word w) /\
-      v_inv asmm impm v w.
+      v_inv pmap v w.
 
-Definition cmd_res_rel (ri: outcome Value unit) (l1: nat) (stck: list word_or_ret) (t1: ASMSemantics.state) (s1: ImpSemantics.state) : Prop :=
+Definition cmd_res_rel (ri: outcome Value unit) (l1: nat)
+  (stck: list word_or_ret) (t1: ASMSemantics.state) (s1: ImpSemantics.state)
+  (pmap: nat -> option (word64 * nat)) : Prop :=
   match ri with
   | Stop (Return v) => exists w,
-    v_inv t1.(memory) s1.(ImpSemantics.memory) v w /\
+    v_inv pmap v w /\
+    mem_inv pmap t1.(memory) s1.(ImpSemantics.memory) /\
     has_stack t1 (Word w :: stck) /\
     t1.(pc) = l1
   | Cont _ =>
@@ -116,14 +123,43 @@ Definition cmd_res_rel (ri: outcome Value unit) (l1: nat) (stck: list word_or_re
   | _ => False
   end.
 
-Definition exp_res_rel (ri: outcome Value Value) (l1: nat) (stck: list word_or_ret) (t1: ASMSemantics.state) (s1: ImpSemantics.state) : Prop :=
+Definition exp_res_rel (ri: outcome Value Value) (l1: nat)
+  (stck: list word_or_ret) (t1: ASMSemantics.state) (s1: ImpSemantics.state)
+  (pmap: nat -> option (word64 * nat)) : Prop :=
   match ri with
   | Cont v => exists w,
-    v_inv t1.(memory) s1.(ImpSemantics.memory) v w /\
+    v_inv pmap v w /\
+    mem_inv pmap t1.(memory) s1.(ImpSemantics.memory) /\
     has_stack t1 (Word w :: stck) /\
     t1.(pc) = l1
   | _ => False
   end.
+
+(* TODO(kπ) test_res_rel *)
+
+(* TODO check if this can be a set *)
+Fixpoint addresses_of (base: word64) (length: nat): list word64 :=
+  match length with
+  | 0 => []
+  | S n => base :: addresses_of (word.add base (word.of_Z 8)) (n)
+  end.
+
+Definition pmap_ok (pmap: nat -> option (word64 * nat)): Prop :=
+  forall p1 p2 base1 len1 base2 len2,
+    pmap p1 = Some (base1, len1) /\ pmap p2 = Some (base2, len2) ->
+    forall addr,
+      List.existsb (word.eqb addr) (addresses_of base1 len1) = true /\
+      List.existsb (word.eqb addr) (addresses_of base2 len2) = true ->
+      p1 = p2.
+
+Definition pmap_subsume (pmap: nat -> option (word64 * nat))
+  (pmap1: nat -> option (word64 * nat)): Prop :=
+  forall p v,
+    pmap p = Some v ->
+    pmap1 p = Some v.
+
+(* relate pmap wiht pmap1, stating that pmap is only ever extended *)
+(* invariant about injectivity of pmap *)
 
 (* Goals *)
 
@@ -132,17 +168,22 @@ Definition goal_exp (e : exp): Prop :=
          (res : outcome Value Value) (t : ASMSemantics.state)
          (vs vs' : v_stack) (fs : f_lookup)
          (asmc : asm_appl) (l1 : nat)
-         (curr rest : list word_or_ret),
+         (curr rest : list word_or_ret)
+         (pmap: nat -> option (word64 * nat)),
     eval_exp e s = (res, s1) ->
     res <> Stop Crash ->
     c_exp e t.(pc) vs = (asmc, l1) ->
     state_rel fs s t ->
-    env_ok s.(vars) vs curr t.(memory) s.(ImpSemantics.memory) ->
+    env_ok s.(vars) vs curr pmap t.(memory) s.(ImpSemantics.memory) ->
     has_stack t (curr ++ rest) ->
+    mem_inv pmap t.(memory) s.(ImpSemantics.memory) ->
+    pmap_ok pmap ->
     odd (List.length rest) = true ->
     code_in t.(pc) (flatten asmc) t.(instructions) ->
-    exists outcome,
+    exists outcome pmap1,
       steps (State t, fuel) outcome /\
+      pmap_ok pmap1 /\
+      pmap_subsume pmap pmap1 /\
       match outcome with
       | (Halt ec output, ck) =>
         prefix output (string_of_list_ascii s1.(ImpSemantics.output)) = true /\
@@ -150,7 +191,38 @@ Definition goal_exp (e : exp): Prop :=
       | (State t1, ck) =>
           state_rel fs s1 t1 /\
           ck = fuel /\
-          exp_res_rel res l1 (curr ++ rest) t1 s1
+          exp_res_rel res l1 (curr ++ rest) t1 s1 pmap1
+      end.
+
+Definition goal_test (tst: test): Prop :=
+  forall (s s1 : ImpSemantics.state) (fuel: nat)
+         (b : bool) (t t1 : ASMSemantics.state)
+         (vs vs' : v_stack) (fs : f_lookup)
+         (asmc : asm_appl) (l1 ltrue lfalse : nat)
+         (curr rest : list word_or_ret)
+         (pmap: nat -> option (word64 * nat)),
+    eval_test tst s = (Cont b, s1) ->
+    c_test_jump tst ltrue lfalse t.(pc) vs = (asmc, l1) ->
+    state_rel fs s t ->
+    env_ok s.(vars) vs curr pmap t.(memory) s.(ImpSemantics.memory) ->
+    has_stack t (curr ++ rest) ->
+    mem_inv pmap t.(memory) s.(ImpSemantics.memory) ->
+    pmap_ok pmap ->
+    odd (List.length rest) = true ->
+    code_in t.(pc) (flatten asmc) t.(instructions) ->
+    exists outcome pmap1,
+      steps (State t, fuel) outcome /\
+      pmap_ok pmap1 /\
+      pmap_subsume pmap pmap1 /\
+      match outcome with
+      | (Halt ec output, ck) =>
+        prefix output (string_of_list_ascii s1.(ImpSemantics.output)) = true /\
+          ec = (word.of_Z 1)
+      | (State t1, ck) =>
+        state_rel fs s1 t1 /\
+        mem_inv pmap1 t1.(memory) s1.(ImpSemantics.memory) /\
+        has_stack t1 (curr ++ rest) /\
+        t1.(pc) = if b then ltrue else lfalse
       end.
 
 Definition goal_cmd (c : cmd): Prop :=
@@ -158,17 +230,22 @@ Definition goal_cmd (c : cmd): Prop :=
          (res : outcome Value unit) (t : ASMSemantics.state)
          (vs vs' : v_stack) (fs : f_lookup)
          (asmc : asm_appl) (l1 : nat)
-         (curr rest : list word_or_ret),
+         (curr rest : list word_or_ret)
+         (pmap: nat -> option (word64 * nat)),
     EVAL_CMD fuel c s = (res, s1) ->
     res <> Stop Crash ->
     c_cmd c t.(pc) fs vs = (asmc, l1, vs') ->
     state_rel fs s t ->
-    env_ok s.(vars) vs curr t.(memory) s.(ImpSemantics.memory) ->
+    env_ok s.(vars) vs curr pmap t.(memory) s.(ImpSemantics.memory) ->
     has_stack t (curr ++ rest) ->
+    mem_inv pmap t.(memory) s.(ImpSemantics.memory) ->
+    pmap_ok pmap ->
     odd (List.length rest) = true ->
     code_in t.(pc) (flatten asmc) t.(instructions) ->
-    exists outcome,
+    exists outcome pmap1,
       steps (State t, fuel) outcome /\
+      pmap_ok pmap1 /\
+      pmap_subsume pmap pmap1 /\
       match outcome with
       | (Halt ec output, ck) =>
           prefix output (string_of_list_ascii s1.(ImpSemantics.output)) = true /\
@@ -176,7 +253,7 @@ Definition goal_cmd (c : cmd): Prop :=
       | (State t1, ck) =>
           state_rel fs s1 t1 /\
           ck = fuel /\
-          cmd_res_rel res l1 (curr ++ rest) t1 s1
+          cmd_res_rel res l1 (curr ++ rest) t1 s1 pmap1
       end.
 
 (* proofs *)
@@ -192,7 +269,9 @@ Ltac cleanup :=
   repeat match goal with
   | [ H: _ /\ _ |- _ ] => destruct H
   | [ H: exists _, _ |- _ ] => destruct H
-  | [ H : True |- _ ] => clear H
+  | [ H: True |- _ ] => clear H
+  | [ H: (_, _) = (_, _) |- _ ] => inversion H; subst; clear H
+  | [ H: _ :: _ = _ :: _ |- _ ] => inversion H; subst; clear H
   end.
 
 Theorem rw_mod_2_even: forall (n: nat),
@@ -413,6 +492,29 @@ Proof.
   end.
 Qed.
 
+Theorem c_test_length: forall tst lt lf l vs c l1,
+  c_test_jump tst lt lf l vs = (c, l1) -> l1 = l + List.length (flatten c).
+Proof.
+  induction tst.
+  all: intros.
+  all: simpl c_test_jump in *.
+  all: repeat match goal with
+  | [ H : context[(if ?x then _ else _)] |- _ ] => destruct x eqn:?
+  | [ H : context [(match ?x with | _ => _ end)] |- _ ] => destruct x eqn:?
+  | [ H : (_, _) = (_, _) |- _ ] => inversion H; subst; clear H
+  | [ |- context[ fst ?x ] ] => destruct x eqn:?; simpl in *
+  | [ H : c_test_jump _ _ _ _ _ = (_, _) |- _ ] => eapply IHtst2 in H; subst
+  | [ H : c_test_jump _ _ _ _ _ = (_, _) |- _ ] => eapply IHtst1 in H; subst
+  | [ H : c_test_jump _ _ _ _ _ = (_, _) |- _ ] => eapply IHtst in H; subst
+  | [ H: c_exp _ _ _ = (_, _) |- _ ] =>
+    eapply c_exp_length in H; subst
+  | _ => progress unfold c_var, c_const, dlet in *
+  | _ => progress simpl in *
+  | _ => progress rewrite length_app
+  | _ => lia
+  end.
+Qed.
+
 Theorem code_in_append: forall xs ys n code,
     code_in n (xs ++ ys) code <->
     (code_in n xs code ∧ code_in (n + List.length xs) ys code).
@@ -493,6 +595,92 @@ Proof.
     all: congruence.
 Qed.
 
+Theorem mem_inv_pmap_subsume: forall pmap pmap1 asmm impm,
+  mem_inv pmap asmm impm ->
+  pmap_subsume pmap pmap1 ->
+  mem_inv pmap1 asmm impm.
+Proof.
+  intros.
+  unfold mem_inv, pmap_subsume in *.
+  intros.
+  eapply H in H1; clear H.
+  cleanup.
+  eexists; eauto.
+  split; eauto.
+  intros.
+  eapply H1 in H2; clear H1.
+  cleanup.
+  eexists; eauto.
+  split; eauto.
+  unfold opt_rel in *.
+  destruct xopt eqn:?; destruct x0 eqn:?.
+  1: unfold v_inv in *; simpl; destruct v0 eqn:?; cleanup; eauto.
+  all: try assumption.
+Qed.
+
+(* Theorem mem_inv_asmm_IMP: forall pmap (impm : list mem_block) asmm asmm1,
+  mem_inv pmap asmm impm ->
+  mem_inv pmap asmm1 impm.
+Proof.
+  unfold mem_inv; intros; cleanup.
+  eapply H in H0; clear H; cleanup.
+  eexists; split; eauto; intros.
+  eapply H0 in H1; clear H0; cleanup.
+  eexists. *)
+
+
+Theorem memory_set_memory: forall s p,
+  memory (set_pc p s) = memory s.
+Proof.
+  intros; simpl; reflexivity.
+Qed.
+
+Theorem env_ok_pmap_subsume: forall vars vs curr pmap pmap1 asmm impm,
+  env_ok vars vs curr pmap asmm impm ->
+  pmap_subsume pmap pmap1 ->
+  env_ok vars vs curr pmap1 asmm impm.
+Proof.
+  intros.
+  unfold env_ok, pmap_subsume in *; cleanup.
+  split; eauto.
+  intros.
+  eapply H1 in H2; clear H1; cleanup.
+  split; eauto.
+  eexists; eauto.
+  split; eauto.
+  unfold v_inv in *; simpl; destruct v eqn:?; cleanup; eauto.
+Qed.
+
+Theorem step_consts: forall s0 s1,
+  step (State s0) (State s1) ->
+  s1.(instructions) = s0.(instructions) ∧
+  ∀w x, read_mem w s0 = Some x -> read_mem w s1 = Some x.
+Proof.
+  inversion 1; intros; eauto.
+  simpl in *; subst.
+  unfold write_mem in *; simpl in *; cleanup.
+  destruct (memory _ _) eqn:?; try destruct o; cleanup.
+  all: inversion H5; clear H5; subst.
+  split; intros; eauto.
+  unfold read_mem in *; simpl in *.
+  destruct (Z.eqb _ _) eqn:?; eauto.
+  rewrite Z.eqb_eq in Heqb; rewrite Heqb in *.
+  destruct (memory s0 w0) eqn:?; subst; eauto; [|inversion H0].
+  assert (w0 = (Naive.wrap (Naive.unsigned wa + Naive.unsigned imm mod Z.pow_pos 2 64))).
+  2: rewrite H0 in *; rewrite Heqo in *; inversion Heqo0.
+Admitted.
+
+Theorem steps_consts:
+  ∀x y,
+    steps x y ->
+    (∀t1 m, y = (State t1,m) -> ∃t0 n, x = (State t0,n)) ∧
+    ∀t0 n t1 m,
+      x = (State t0,n) ∧ y = (State t1,m) ->
+      t1.(instructions) = t0.(instructions) ∧
+      ∀w x, read_mem w t0 = Some x -> read_mem w t1 = Some x.
+Proof.
+Admitted.
+
 Theorem steps_instructions: forall s1 s2 f1 f2,
   steps (State s1, f1) (State s2, f2) -> s1.(instructions) = s2.(instructions).
 Proof.
@@ -534,9 +722,10 @@ Ltac crunch_give_up_even :=
   | _ => tauto
 end.
 
-Theorem env_ok_add_None: forall vars vs curr x asmm impm,
-  env_ok vars vs curr asmm impm ->
-  env_ok vars (None :: vs) (Word x :: curr) asmm impm.
+Theorem env_ok_add_None: forall vars vs curr x asmm impm pmap pmap1,
+  env_ok vars vs curr pmap asmm impm ->
+  pmap_subsume pmap pmap1 ->
+  env_ok vars (None :: vs) (Word x :: curr) pmap1 asmm impm.
 Proof.
   intros * H.
   unfold env_ok in *; cleanup.
@@ -548,10 +737,33 @@ Proof.
   all: simpl.
   all: try rewrite index_of_spec; try lia.
   all: unfold v_inv in *.
-  1: simpl; eapply H2.
+  1: simpl; eapply H3.
   destruct v; [assumption|].
-  assumption.
+  cleanup.
+  unfold pmap_subsume in *.
+  eapply H1 in H4.
+  eauto.
 Qed.
+
+Theorem pmap_subsume_refl: forall pmap,
+  pmap_subsume pmap pmap.
+Proof.
+  unfold pmap_subsume; intros; assumption.
+Qed.
+
+Theorem pmap_subsume_trans: forall pmap1 pmap2 pmap3,
+  pmap_subsume pmap1 pmap2 ->
+  pmap_subsume pmap2 pmap3 ->
+    pmap_subsume pmap1 pmap3.
+Proof.
+  unfold pmap_subsume; intros; eauto.
+Qed.
+
+Theorem mul_div_id: forall n m,
+  n mod m = 0 ->
+  n / m * m = n.
+Proof.
+Admitted.
 
 Ltac rw tac :=
   let n := fresh "H" in
@@ -560,6 +772,24 @@ Ltac rw tac :=
 Ltac rwr tac :=
   let n := fresh "H" in
   ltac:(tac); intros n; rewrite <- n in *; clear n.
+
+Ltac apply_IEnv_lookup :=
+  match goal with
+  | [ H1 : IEnv.lookup _ _ = _, H2: context[IEnv.lookup _ _] |- _ ] =>
+    eapply H2 in H1; cleanup
+  end.
+
+Ltac apply_lookup_fun :=
+  match goal with
+  | [ H1 : lookup_fun _ _ = _, H2: context[lookup_fun _ _] |- _ ] =>
+    eapply H2 in H1; cleanup
+  end.
+
+Ltac eval_exp_contr_stop_tac :=
+  lazymatch goal with
+  | [ H: eval_exp _ _ = (Stop ?v, _) |- _ ] =>
+    exfalso; destruct v eqn:?; eapply eval_exp_not_stop in H; eauto; try congruence
+  end.
 
 Theorem c_exp_Const : forall (w: word64),
   goal_exp (ImpSyntax.Const w).
@@ -573,54 +803,29 @@ Proof.
   unfold state_rel in *; cleanup.
   unfold env_ok in *; cleanup.
   simpl c_exp in *; unfold c_const in *.
-  destruct (word.of_Z _ <w _) eqn:?.
-  1: {
-    eexists.
-    inversion H1; subst; clear H1.
-    simpl flatten in *.
-    split.
-    - eapply steps_trans.
-      + eapply steps_step_same.
-        simpl code_in in *; cleanup.
-        eapply step_jump; eauto.
-        constructor.
-      + simpl.
-        all: unfold state_rel in *; cleanup.
-        eapply give_up.
-        all: unfold_stack; eauto.
-        unfold env_ok in *; cleanup.
-        crunch_give_up_even.
-    - simpl.
-      split; try reflexivity.
-      inversion H; subst.
-      unfold state_rel in *; cleanup.
-      rewrite <- H10.
-      rewrite prefix_correct.
-      apply substring_noop.
-  }
-  inversion H1; subst; clear H1.
+  cleanup.
   simpl flatten in *.
-  eexists.
+  eexists; eexists.
   split.
   1: {
     eapply steps_trans.
-    + eapply steps_step_same.
-      simpl code_in in *; cleanup.
-      eapply step_push in e; eauto.
-    + eapply steps_step_same.
-      simpl code_in in *; cleanup.
-      eapply step_const with (w := w).
-      eauto.
+    1: eapply steps_step_same.
+    1: simpl code_in in *; cleanup.
+    1: eapply step_push in e; eauto.
+    eapply steps_step_same.
+    simpl code_in in *; cleanup.
+    eapply step_const.
+    eauto.
   }
   simpl.
   repeat split; unfold state_rel in *; cleanup; intros; repeat split; simpl.
   all: inversion H; subst; eauto.
+  - apply pmap_subsume_refl.
   - unfold code_rel in *.
     cleanup.
     eauto.
   - unfold code_rel in *; cleanup.
-    eapply H11 in H1.
-    cleanup.
+    apply_lookup_fun.
     eexists.
     split; eauto.
   - eexists; eexists.
@@ -628,10 +833,9 @@ Proof.
   - unfold exp_res_rel.
     eexists.
     repeat split.
-    1: eapply w_lt_bound; eauto.
+    + simpl; assumption.
     + unfold has_stack.
-      simpl.
-      eauto.
+      simpl; eauto.
     + simpl.
       lia.
 Qed.
@@ -650,8 +854,8 @@ Proof.
   simpl c_exp in *; unfold c_var in *; unfold dlet in *.
   destruct (index_of n 0 vs =? 0) eqn:?.
   1: {
-    eexists.
-    inversion H1; subst; clear H1.
+    eexists; eexists.
+    cleanup.
     simpl flatten in *.
     split.
     - eapply steps_step_same.
@@ -661,41 +865,33 @@ Proof.
       destruct (IEnv.lookup (vars s) n) eqn:?; unfold_outcome; inversion H; subst.
       2: unfold not in H0; contradiction.
       repeat split; simpl; eauto.
+      1: eapply pmap_subsume_refl.
       1: eexists; eexists; eauto.
       unfold v_inv, has_stack.
-      destruct v eqn:?.
+      destruct v eqn:?; subst.
       1: {
         assert (x = w).
         1: {
-          eapply H16 in Heqo; cleanup; subst.
+          eapply H18 in Heqo; cleanup; subst.
           unfold v_inv in *; cleanup; subst.
           rewrite Nat.eqb_eq in *.
           rewrite Heqb in *.
-          destruct curr; inversion H8; subst.
+          destruct curr; inversion H10; subst.
           inversion H4; subst.
           reflexivity.
         }
         subst.
-        exists w; repeat split; try exists w.
-        all: try eexists; repeat split.
-        all: unfold_stack.
-        all: eauto.
-        unfold v_inv in *; cleanup; subst.
-        unfold env_ok in *; cleanup.
-        pose (H16 n (ImpSyntax.Word w) Heqo); cleanup.
-        unfold v_inv in *; cleanup.
-        eapply w_lt_bound; eauto.
+        exists w; repeat split; eauto.
       }
+      apply_IEnv_lookup; unfold v_inv in *; cleanup.
       eexists; repeat split.
+      2: assumption.
       all: repeat eexists; repeat split.
-      all: unfold_stack.
-      all: eauto.
-      unfold env_ok in *; cleanup.
-      eapply H16 in Heqo; cleanup; subst.
-      unfold v_inv in *; cleanup; subst.
+      1: eauto.
+      all: simpl; eauto.
       rewrite Nat.eqb_eq in *.
       rewrite Heqb in *.
-      destruct curr; inversion H8; subst.
+      destruct curr; inversion H10; subst.
       inversion H4; subst.
       assumption.
   }
@@ -703,60 +899,68 @@ Proof.
   unfold lookup_var in *; cleanup.
   destruct (IEnv.lookup (vars s) n) eqn:?; unfold_outcome; inversion H; subst.
   2: unfold not in H0; contradiction.
-  pose (H16 n v Heqo); cleanup.
-  eexists.
-  inversion H1; subst; clear H1.
+  apply_IEnv_lookup; cleanup.
+  eexists; eexists.
   simpl flatten in *.
   split.
   - eapply steps_trans.
-    + eapply steps_step_same.
-      simpl code_in in *; cleanup.
-      eapply step_push in e; eauto.
-    + eapply steps_step_same.
-      rewrite Nat.eqb_neq in *.
-      simpl code_in in *; cleanup.
-      eapply step_load_rsp; eauto.
-      all: unfold_stack; eauto.
-      2: {
-        rewrite <- H4 in *.
-        rewrite nth_error_app.
-        rewrite <- Nat.ltb_lt in *.
-        rewrite H8.
-        rewrite H18.
-        reflexivity.
-      }
-      eapply Nat.lt_trans; [eauto|].
-      assert (List.length (curr ++ rest) = List.length (Word x :: stack t)); [rewrite H4; reflexivity|].
-      rewrite length_app in *.
-      rewrite length_cons in *.
-      rewrite <- H1.
-      destruct rest; [inversion H5|].
-      rewrite length_cons in *.
-      lia.
+    1: eapply steps_step_same.
+    1: simpl code_in in *; cleanup.
+    1: eapply step_push in e; eauto.
+    eapply steps_step_same.
+    rewrite Nat.eqb_neq in *.
+    simpl code_in in *; cleanup.
+    eapply step_load_rsp; eauto.
+    all: unfold_stack; eauto.
+    2: {
+      rewrite <- H4 in *.
+      rewrite nth_error_app.
+      rewrite <- Nat.ltb_lt in *.
+      rewrite H1.
+      eauto.
+    }
+    eapply Nat.lt_trans; [eauto|].
+    assert (List.length (curr ++ rest) = List.length (Word x :: stack t)); [rewrite H4; reflexivity|].
+    rewrite length_app in *.
+    rewrite length_cons in *.
+    rewrite <- H.
+    destruct rest; [inversion H7|].
+    rewrite length_cons in *.
+    lia.
   - simpl.
     unfold state_rel in *; cleanup.
     unfold code_rel in *; cleanup.
     repeat split; simpl; eauto.
+    1: eapply pmap_subsume_refl.
     1: eexists; eexists; eauto.
-    unfold v_inv, has_stack.
+    unfold v_inv, has_stack in *.
     destruct v eqn:?.
     1: {
-      eexists; repeat split; try eexists.
-      all: try eexists; repeat split.
-      all: unfold_stack.
-      all: eauto; try lia.
-      - unfold v_inv in *; cleanup; subst.
-        eapply w_lt_bound; eauto.
-      - eapply H16 in Heqo; cleanup; subst.
-        unfold v_inv in *; cleanup; subst.
-        reflexivity.
+      unfold v_inv in *; cleanup.
+      eexists; repeat split.
+      1: assumption.
+      2: lia.
+      repeat eexists; repeat split.
+      all: simpl; eauto.
+      subst; eauto.
     }
+    cleanup.
     eexists; repeat split.
+    2: assumption.
+    3: lia.
     all: repeat eexists; repeat split.
-    all: unfold_stack.
-    all: eauto.
-    lia.
+    all: simpl; eauto.
 Qed.
+
+Ltac bin_exp_post_tac :=
+  simpl;
+  repeat split; eauto;
+  unfold code_rel in *; cleanup; eauto;
+  [try eapply pmap_subsume_trans; eauto|..];
+  [eexists; eexists; eauto|..];
+  eexists; repeat split; eauto; repeat eexists;
+  try rewrite Z.add_comm; try reflexivity;
+  try lia.
 
 Theorem c_exp_Add : forall (e1 e2: exp),
   goal_exp e1 -> goal_exp e2 ->
@@ -765,137 +969,73 @@ Proof.
   intros.
   unfold goal_exp; intros.
   simpl eval_exp in *.
-  simpl c_exp in *; unfold c_add in *; unfold dlet in *.
+  simpl c_exp in *; unfold c_add, c_sub, c_div, c_load in *; unfold dlet in *.
   destruct (eval_exp e1 s) eqn:?; simpl in *; unfold bind at 1 in H1; rewrite Heqp in *; subst.
   destruct o eqn:?; subst.
-  2: {
-    destruct v eqn:?; subst.
-    all: inversion H1; subst.
-    all: eapply eval_exp_not_stop in Heqp; unfold not in *; eauto; exfalso; apply Heqp; eauto.
-  }
+  2: eval_exp_contr_stop_tac.
   destruct (eval_exp e2 s0) eqn:?; simpl in *; unfold bind at 1 in H1; rewrite Heqp0 in H1; subst.
   destruct o eqn:?; subst.
-  2: {
-    destruct v eqn:?; subst.
-    all: inversion H1; subst.
-    all: eapply eval_exp_not_stop in Heqp0; unfold not in *; eauto; exfalso; apply Heqp0; eauto.
-  }
+  2: eval_exp_contr_stop_tac.
   unfold combine_word in *.
-  destruct v eqn:?.
-  2: inversion H1; subst; contradiction.
-  destruct v0 eqn:?.
-  2: inversion H1; subst; contradiction.
-  unfold_outcome; inversion H1; subst.
+  destruct v eqn:?; unfold_outcome; cleanup; subst.
+  2: contradiction.
+  destruct v0 eqn:?; unfold_outcome; cleanup; subst.
+  2: contradiction.
   destruct (c_exp e1 (pc t) vs) eqn:?; simpl in *.
   destruct (c_exp e2 n (None :: vs)) eqn:?; simpl in *.
   specialize (eval_exp_pure e1 _ _ _ Heqp).
   specialize (eval_exp_pure e2 _ _ _ Heqp0).
   intros; subst.
-  unfold goal_exp in H; eapply H in Heqp; clear H; eauto; inversion H3; subst.
+  unfold goal_exp in H; eapply H in Heqp; clear H; eauto.
   all: simpl flatten in *.
   all: repeat rewrite code_in_append in *; cleanup.
   all: try congruence.
   rwr ltac:(specialize (c_exp_length e1 _ _ _ _ Heqp1)).
   specialize (c_exp_length e2 _ _ _ _ Heqp2) as ?; subst.
-  destruct x; destruct s; cleanup.
-  2: eexists; split; eauto; simpl; split; eauto.
-  unfold exp_res_rel in *; cleanup.
+  destruct x; destruct s; cleanup; subst.
+  2: repeat eexists; repeat split; eauto; simpl; split; eauto.
+  unfold exp_res_rel in *; cleanup; subst.
   unfold goal_exp in H0.
-  rewrite <- H15 in *.
   rw ltac:(specialize (steps_instructions _ _ _ _ H10)).
   eapply H0 in Heqp0; clear H0; eauto; inversion H3; clear H3; subst; cleanup; eauto.
   2: congruence.
-  1: destruct x0; destruct s0; cleanup; subst.
-  2: eexists; split; [eapply steps_trans|]; eauto; simpl; split; eauto.
+  1: destruct x1; destruct s0; cleanup; subst.
+  2: repeat eexists; repeat split; [eapply steps_trans|..]; eauto; simpl; eauto.
+  2: eapply pmap_subsume_trans; eauto.
   all: unfold exp_res_rel in *; cleanup.
-  1: instantiate (1 := (Word x :: curr)) in H15; simpl in *; cleanup.
+  all: try rewrite <- H24 in *.
+  all: unfold state_rel in *; cleanup.
+  1: instantiate (1 := (Word w :: curr)) in H23.
+  all: simpl in *; cleanup; subst.
   1: {
-    unfold state_rel in *; cleanup.
     specialize (has_stack_even t (curr ++ rest) H6) as ?.
-    specialize (has_stack_even _ _ H14) as ?.
-    specialize (has_stack_even _ _ H15) as ?.
-    unfold has_stack in *; cleanup; subst.
+    specialize (has_stack_even _ _ H16) as ?.
+    specialize (has_stack_even _ _ H23) as ?.
+    unfold has_stack in *; cleanup.
     unfold env_ok in *; cleanup.
-    inversion H15; clear H15; subst.
-    inversion H14; clear H14; subst.
-    rw ltac:(specialize (steps_instructions _ _ _ _ H0)).
-    destruct (word.ltu ((word.of_Z (2 ^ 63 - 1)): word64)
-      (Naive.wrap ((Naive.unsigned x7) + (Naive.unsigned x9)))) eqn:?.
-    1: {
-      eexists.
-      split.
-      1: {
-        eapply steps_trans.
-        1: eapply H10.
-        eapply steps_trans.
-        1: eapply H0.
-        rewrite <- H16 in *.
-        unfold code_in in H9; cleanup; subst.
-        eapply steps_trans.
-        1: eapply steps_step_same.
-        1: eapply step_pop; eauto.
-        eapply steps_trans.
-        1: eapply steps_step_same.
-        1: eapply step_add; eauto.
-        1: unfold_stack; eauto.
-        eapply steps_trans.
-        1: eapply steps_step_same.
-        1: eapply step_jump; eauto.
-        1: unfold_stack; constructor; eauto.
-        1: simpl; eauto.
-        simpl Z.pow in *; unfold Z.pow_pos in *; simpl PosDef.Pos.iter in *; simpl Z.sub in *.
-        rewrite Heqb.
-        unfold_stack.
-        eapply give_up; unfold_stack; eauto.
-        crunch_give_up_even.
-      }
-      simpl.
-      repeat split; eauto.
-      rewrite H21.
-      rewrite prefix_correct.
-      apply substring_noop.
-    }
-    eexists.
+    rw ltac:(specialize (steps_instructions _ _ _ _ H3)).
+    eexists; eexists.
     split.
     1: {
       eapply steps_trans.
       1: eapply H10.
       eapply steps_trans.
-      1: eapply H0.
-      rewrite <- H16 in *.
-      unfold code_in in H9; cleanup; subst.
+      1: eapply H3.
       eapply steps_trans.
       1: eapply steps_step_same.
-      1: eapply step_pop; [eapply H9|]; eauto.
+      1: eapply step_pop; eauto.
       eapply steps_trans.
       1: eapply steps_step_same.
       1: eapply step_add; eauto.
       1: unfold_stack; eauto.
-      eapply steps_trans.
-      1: eapply steps_step_same.
-      1: eapply step_jump; eauto.
-      1: unfold_stack; constructor; eauto.
-      1: simpl; eauto.
-      simpl Z.pow in *; unfold Z.pow_pos in *; simpl PosDef.Pos.iter in *; simpl Z.sub in *.
-      rewrite Heqb.
       eapply steps_refl.
     }
-    simpl.
-    repeat split; eauto.
-    all: unfold code_rel in *; cleanup; eauto.
-    1: eexists; eexists; eauto.
-    eexists; repeat split; repeat eexists; eauto.
-    3: rewrite H16; lia.
-    2: rewrite Z.add_comm; reflexivity.
-    unfold v_inv in *; cleanup; subst.
-    eapply z_lt_bound.
-    rewrite Z.add_comm; assumption.
+    bin_exp_post_tac.
   }
   all: eauto.
   unfold state_rel in *; cleanup.
   eapply env_ok_add_None; eauto.
-  admit.
-Admitted.
+Qed.
 
 Theorem c_exp_Sub : forall (e1 e2: exp),
   goal_exp e1 -> goal_exp e2 ->
@@ -904,127 +1044,64 @@ Proof.
   intros.
   unfold goal_exp; intros.
   simpl eval_exp in *.
-  simpl c_exp in *; unfold c_sub in *; unfold dlet in *.
+  simpl c_exp in *; unfold c_add, c_sub, c_div, c_load in *; unfold dlet in *.
   destruct (eval_exp e1 s) eqn:?; simpl in *; unfold bind at 1 in H1; rewrite Heqp in *; subst.
   destruct o eqn:?; subst.
-  2: {
-    destruct v eqn:?; subst.
-    all: inversion H1; subst.
-    all: eapply eval_exp_not_stop in Heqp; unfold not in *; eauto; exfalso; apply Heqp; eauto.
-  }
+  2: eval_exp_contr_stop_tac.
   destruct (eval_exp e2 s0) eqn:?; simpl in *; unfold bind at 1 in H1; rewrite Heqp0 in H1; subst.
   destruct o eqn:?; subst.
-  2: {
-    destruct v eqn:?; subst.
-    all: inversion H1; subst.
-    all: eapply eval_exp_not_stop in Heqp0; unfold not in *; eauto; exfalso; apply Heqp0; eauto.
-  }
+  2: eval_exp_contr_stop_tac.
   unfold combine_word in *.
-  destruct v eqn:?.
-  2: inversion H1; subst; contradiction.
-  destruct v0 eqn:?.
-  2: inversion H1; subst; contradiction.
-  unfold_outcome; inversion H1; subst.
+  destruct v eqn:?; unfold_outcome; cleanup; subst.
+  2: contradiction.
+  destruct v0 eqn:?; unfold_outcome; cleanup; subst.
+  2: contradiction.
   destruct (c_exp e1 (pc t) vs) eqn:?; simpl in *.
   destruct (c_exp e2 n (None :: vs)) eqn:?; simpl in *.
   specialize (eval_exp_pure e1 _ _ _ Heqp).
   specialize (eval_exp_pure e2 _ _ _ Heqp0).
   intros; subst.
-  unfold goal_exp in H; eapply H in Heqp; clear H; eauto; inversion H3; subst.
+  unfold goal_exp in H; eapply H in Heqp; clear H; eauto.
   all: simpl flatten in *.
   all: repeat rewrite code_in_append in *; cleanup.
   all: try congruence.
   rwr ltac:(specialize (c_exp_length e1 _ _ _ _ Heqp1)).
   specialize (c_exp_length e2 _ _ _ _ Heqp2) as ?; subst.
-  destruct x; destruct s; cleanup.
-  2: eexists; split; eauto; simpl; split; eauto.
-  unfold exp_res_rel in *; cleanup.
+  destruct x; destruct s; cleanup; subst.
+  2: repeat eexists; repeat split; eauto; simpl; split; eauto.
+  unfold exp_res_rel in *; cleanup; subst.
   unfold goal_exp in H0.
-  rewrite <- H15 in *.
   rw ltac:(specialize (steps_instructions _ _ _ _ H10)).
   eapply H0 in Heqp0; clear H0; eauto; inversion H3; clear H3; subst; cleanup; eauto.
   2: congruence.
-  1: destruct x0; destruct s0; cleanup; subst.
-  2: eexists; split; [eapply steps_trans|]; eauto; simpl; split; eauto.
+  1: destruct x1; destruct s0; cleanup; subst.
+  2: repeat eexists; repeat split; [eapply steps_trans|..]; eauto; simpl; eauto.
+  2: eapply pmap_subsume_trans; eauto.
   all: unfold exp_res_rel in *; cleanup.
-  1: instantiate (1 := (Word x :: curr)) in H15; simpl in *; cleanup.
+  all: try rewrite <- H24 in *.
+  all: unfold state_rel in *; cleanup.
+  1: instantiate (1 := (Word w :: curr)) in H23.
+  all: simpl in *; cleanup; subst.
   1: {
-    unfold state_rel in *; cleanup.
     specialize (has_stack_even t (curr ++ rest) H6) as ?.
-    specialize (has_stack_even _ _ H14) as ?.
-    specialize (has_stack_even _ _ H15) as ?.
-    unfold has_stack in *; cleanup; subst.
+    specialize (has_stack_even _ _ H16) as ?.
+    specialize (has_stack_even _ _ H23) as ?.
+    unfold has_stack in *; cleanup.
     unfold env_ok in *; cleanup.
-    inversion H15; clear H15; subst.
-    inversion H14; clear H14; subst.
-    rw ltac:(specialize (steps_instructions _ _ _ _ H0)).
-    destruct (word.ltu x7 x9) eqn:?.
-    1: {
-      eexists.
-      split.
-      1: {
-        eapply steps_trans.
-        1: eapply H10.
-        eapply steps_trans.
-        1: eapply H0.
-        rewrite <- H16 in *.
-        unfold code_in in H9; cleanup; subst.
-        eapply steps_trans.
-        1: eapply steps_step_same.
-        1: eapply step_pop; eauto.
-        eapply steps_trans.
-        1: eapply steps_step_same.
-        1: eapply step_jump; eauto.
-        1: constructor; simpl; eauto.
-        rewrite Heqb.
-        eapply steps_trans.
-        1: eapply steps_step_same.
-        1: eapply step_sub; eauto.
-        1: assert (pc s0 + 3 = pc s0 + 1 + 1 + 1) as -> by lia.
-        1: unfold_stack; eauto.
-        1-2: simpl; eauto.
-        eapply steps_trans.
-        1: eapply steps_step_same.
-        1: eapply step_mov; eauto.
-        1: assert (pc s0 + 3 = pc s0 + 1 + 1 + 1) as -> by lia.
-        1: unfold_stack; eauto.
-        1: simpl; eauto.
-        eapply steps_refl.
-      }
-      simpl.
-      repeat split; eauto.
-      all: unfold code_rel in *; cleanup; eauto.
-      1: eexists; eexists; eauto.
-      eexists; repeat split; repeat eexists; eauto.
-      2: lia.
-      rewrite word.unsigned_ltu in *.
-      eapply sub_lt_bound; eauto.
-    }
-    eexists.
+    rw ltac:(specialize (steps_instructions _ _ _ _ H3)).
+    eexists; eexists.
     split.
     1: {
       eapply steps_trans.
       1: eapply H10.
       eapply steps_trans.
-      1: eapply H0.
-      rewrite <- H16 in *.
-      unfold code_in in H9; cleanup; subst.
+      1: eapply H3.
       eapply steps_trans.
       1: eapply steps_step_same.
       1: eapply step_pop; eauto.
       eapply steps_trans.
       1: eapply steps_step_same.
-      1: eapply step_jump; eauto.
-      1: constructor; simpl; eauto.
-      rewrite Heqb.
-      eapply steps_trans.
-      1: eapply steps_step_same.
-      1: eapply step_mov; eauto.
-      1: simpl; eauto.
-      eapply steps_trans.
-      1: eapply steps_step_same.
       1: eapply step_sub; eauto.
-      1: unfold_stack; eauto.
       1: simpl; eauto.
       eapply steps_trans.
       1: eapply steps_step_same.
@@ -1032,23 +1109,875 @@ Proof.
       1: simpl; eauto.
       eapply steps_refl.
     }
-    simpl.
-    repeat split; eauto.
-    all: unfold code_rel in *; cleanup; eauto.
-    1: eexists; eexists; eauto.
-    eexists; repeat split; repeat eexists; eauto.
-    3: lia.
-    1: admit. (* ((Naive.unsigned x9 - Naive.unsigned x7) mod Z.pow_pos 2 64 <?
-Z.pow_pos 2 63 mod Z.pow_pos 2 64)%Z = true *)
-    admit. (* Some (Naive.wrap (Naive.unsigned x9 - Naive.unsigned x9)) =
-Some (Naive.wrap (Naive.unsigned x9 - Naive.unsigned x7)) *)
+    bin_exp_post_tac.
   }
   all: eauto.
   unfold state_rel in *; cleanup.
   eapply env_ok_add_None; eauto.
-  admit.
+Qed.
+
+Theorem c_exp_Div : forall (e1 e2: exp),
+  goal_exp e1 -> goal_exp e2 ->
+  goal_exp (ImpSyntax.Div e1 e2).
+Proof.
+  intros.
+  unfold goal_exp; intros.
+  simpl eval_exp in *.
+  simpl c_exp in *; unfold c_add, c_sub, c_div, c_load in *; unfold dlet in *.
+  destruct (eval_exp e1 s) eqn:?; simpl in *; unfold bind at 1 in H1; rewrite Heqp in *; subst.
+  destruct o eqn:?; subst.
+  2: eval_exp_contr_stop_tac.
+  destruct (eval_exp e2 s0) eqn:?; simpl in *; unfold bind at 1 in H1; rewrite Heqp0 in H1; subst.
+  destruct o eqn:?; subst.
+  2: eval_exp_contr_stop_tac.
+  unfold combine_word in *.
+  destruct (value_eqb _ _) eqn:?; unfold_outcome; cleanup; subst.
+  1: contradiction.
+  destruct v eqn:?; unfold_outcome; cleanup; subst.
+  2: contradiction.
+  destruct v0 eqn:?; unfold_outcome; cleanup; subst.
+  2: contradiction.
+  unfold value_eqb in *.
+  rewrite word.unsigned_eqb in *; simpl word.unsigned in *; rewrite Z.mod_0_l in *; [|lia].
+  rewrite Heqb in *.
+  destruct (c_exp e1 (pc t) vs) eqn:?; simpl in *.
+  destruct (c_exp e2 n (None :: vs)) eqn:?; simpl in *.
+  specialize (eval_exp_pure e1 _ _ _ Heqp).
+  specialize (eval_exp_pure e2 _ _ _ Heqp0).
+  intros; subst.
+  unfold goal_exp in H; eapply H in Heqp; clear H; eauto.
+  all: simpl flatten in *.
+  all: repeat rewrite code_in_append in *; cleanup.
+  all: try congruence.
+  rwr ltac:(specialize (c_exp_length e1 _ _ _ _ Heqp1)).
+  specialize (c_exp_length e2 _ _ _ _ Heqp2) as ?; subst.
+  destruct x; destruct s; cleanup; subst.
+  2: repeat eexists; repeat split; eauto; simpl; split; eauto.
+  unfold exp_res_rel in *; cleanup; subst.
+  rw ltac:(specialize (steps_instructions _ _ _ _ H10)).
+  unfold goal_exp in H0.
+  eapply H0 in Heqp0; clear H0; eauto; inversion H3; clear H3; subst; cleanup; eauto.
+  2: congruence.
+  1: destruct x1; destruct s0; cleanup; subst.
+  2: repeat eexists; repeat split; [eapply steps_trans|..]; eauto; simpl; eauto.
+  2: eapply pmap_subsume_trans; eauto.
+  all: unfold exp_res_rel in *; cleanup.
+  all: try rewrite <- H24 in *.
+  all: unfold state_rel in *; cleanup.
+  1: instantiate (1 := (Word w :: curr)) in H23.
+  all: simpl in *; cleanup; subst.
+  1: {
+    specialize (has_stack_even t (curr ++ rest) H6) as ?.
+    specialize (has_stack_even _ _ H16) as ?.
+    specialize (has_stack_even _ _ H23) as ?.
+    unfold has_stack in *; cleanup.
+    unfold env_ok in *; cleanup.
+    rw ltac:(specialize (steps_instructions _ _ _ _ H3)).
+    eexists; eexists.
+    split.
+    1: {
+      eapply steps_trans.
+      1: eapply H10.
+      eapply steps_trans.
+      1: eapply H3.
+      eapply steps_trans.
+      1: eapply steps_step_same.
+      1: eapply step_mov; eauto.
+      eapply steps_trans.
+      1: eapply steps_step_same.
+      1: eapply step_pop; eauto.
+      1: simpl; eauto.
+      eapply steps_trans.
+      1: eapply steps_step_same.
+      1: eapply step_const; eauto.
+      eapply steps_trans.
+      1: eapply steps_step_same.
+      1: eapply step_div; eauto.
+      2: simpl; eauto.
+      2: simpl; eauto.
+      1: unfold not; intros ->; rewrite Z.eqb_neq in *; eapply Heqb.
+      1: simpl; rewrite Z.mod_0_l; try reflexivity; lia.
+      eapply steps_refl.
+    }
+    bin_exp_post_tac.
+    rewrite Heqb; reflexivity.
+  }
+  all: eauto.
+  unfold state_rel in *; cleanup.
+  eapply env_ok_add_None; eauto.
+Qed.
+
+Theorem c_exp_Read : forall (e1 e2: exp),
+  goal_exp e1 -> goal_exp e2 ->
+  goal_exp (ImpSyntax.Read e1 e2).
+Proof.
+  intros.
+  unfold goal_exp; intros.
+  simpl eval_exp in *; simpl mem_load in *.
+  simpl c_exp in *; unfold c_add, c_sub, c_div, c_load in *; unfold dlet in *.
+  destruct (eval_exp e1 s) eqn:?; simpl in *; unfold bind at 1 in H1; rewrite Heqp in *; subst.
+  destruct o eqn:?; subst.
+  2: eval_exp_contr_stop_tac.
+  destruct (eval_exp e2 s0) eqn:?; simpl in *; unfold bind at 1 in H1; rewrite Heqp0 in H1; subst.
+  destruct o eqn:?; subst.
+  2: eval_exp_contr_stop_tac.
+  unfold mem_load in *.
+  destruct v eqn:?; unfold_outcome; cleanup; subst.
+  1: contradiction.
+  destruct v0 eqn:?; unfold_outcome; cleanup; subst.
+  2: contradiction.
+  destruct (negb (_)) eqn:?; unfold_outcome; cleanup; subst.
+  1: contradiction.
+  destruct (nth_error _ _) eqn:?; unfold_outcome; cleanup; subst.
+  2: contradiction.
+  destruct (nth_error l _) eqn:?; unfold_outcome; cleanup; subst.
+  2: contradiction.
+  destruct o eqn:?; unfold_outcome; cleanup; subst.
+  2: contradiction.
+  rewrite negb_false_iff in *; rewrite Nat.eqb_eq in *.
+  Opaque Nat.modulo.
+  Opaque Nat.div.
+  destruct (c_exp e1 (pc t) vs) eqn:?; simpl in *.
+  destruct (c_exp e2 n (None :: vs)) eqn:?; simpl in *.
+  specialize (eval_exp_pure e1 _ _ _ Heqp).
+  specialize (eval_exp_pure e2 _ _ _ Heqp0).
+  intros; subst.
+  unfold goal_exp in H; eapply H in Heqp; clear H; eauto.
+  all: repeat rewrite code_in_append in *; cleanup.
+  all: try congruence.
+  rwr ltac:(specialize (c_exp_length e1 _ _ _ _ Heqp1)).
+  specialize (c_exp_length e2 _ _ _ _ Heqp2) as ?; subst.
+  destruct x; destruct s; cleanup; subst.
+  2: repeat eexists; repeat split; eauto; simpl; split; eauto.
+  unfold exp_res_rel in *; cleanup; subst.
+  rw ltac:(specialize (steps_instructions _ _ _ _ H10)).
+  unfold goal_exp in H0.
+  eapply H0 in Heqp0; clear H0; eauto; inversion H3; clear H3; subst; cleanup; eauto.
+  2: congruence.
+  1: destruct x1; destruct s0; cleanup; subst.
+  2: repeat eexists; repeat split; [eapply steps_trans|..]; eauto; simpl; eauto.
+  2: eapply pmap_subsume_trans; eauto.
+  all: unfold exp_res_rel in *; cleanup.
+  all: try rewrite <- H24 in *.
+  all: unfold state_rel in *; cleanup.
+  1: instantiate (1 := (Word x :: curr)) in H23.
+  all: simpl in *; cleanup; subst.
+  1: {
+    specialize (has_stack_even t (curr ++ rest) H6) as ?.
+    specialize (has_stack_even _ _ H16) as ?.
+    specialize (has_stack_even _ _ H23) as ?.
+    unfold has_stack in *; cleanup.
+    unfold env_ok in *; cleanup.
+    rw ltac:(specialize (steps_instructions _ _ _ _ H3)).
+    eapply mem_inv_pmap_subsume with (pmap1 := x2) in H7.
+    2: eapply pmap_subsume_trans; eauto.
+    eapply H22 in Heqo; cleanup.
+    eapply H34 in Heqo0; clear H34; cleanup.
+    unfold opt_rel in *; destruct x10; try contradiction.
+    eexists; eexists.
+    split.
+    1: {
+      eapply steps_trans.
+      1: eauto.
+      eapply steps_trans.
+      1: eauto.
+      eapply steps_trans.
+      1: eapply steps_step_same.
+      1: eapply step_pop; eauto.
+      eapply steps_trans.
+      1: eapply steps_step_same.
+      1: eapply step_add; eauto.
+      1: simpl; eauto.
+      eapply steps_trans.
+      1: eapply steps_step_same.
+      1: eapply step_load; eauto.
+      1: simpl; eauto.
+      2: eapply steps_refl.
+      simpl in *.
+      unfold_stack; unfold read_mem; simpl.
+      assert (
+        (Naive.wrap (Naive.unsigned x + Z.of_nat (w2n x1 / 8 * 8) mod Z.pow_pos 2 64)) =
+        (Naive.wrap
+          ((Naive.unsigned x11 + Naive.unsigned x1) mod Z.pow_pos 2 64 +
+          (0 mod Z.pow_pos 2 4) mod Z.pow_pos 2 64))
+      ) as <-.
+      2: rewrite H34; eauto.
+      eapply H19 in H14; rewrite H14 in *; cleanup.
+      inversion H23; subst.
+      unfold w2n; simpl.
+      cbn.
+      rewrite mul_div_id; eauto.
+      rewrite Z2Nat.id.
+      2: admit. (* 0 <= Naive.unsigned*)
+      rewrite Z.add_0_r.
+      rewrite Naive._unsigned_in_range at 1.
+      Search (word.wrap).
+      admit. (* Naive.wrap (Naive.unsigned x + Naive.unsigned x1) =
+        Naive.wrap ((Naive.unsigned x + Naive.unsigned x1) mod 18446744073709551616) *)
+    }
+    bin_exp_post_tac.
+  }
+  all: eauto.
+  unfold state_rel in *; cleanup.
+  eapply env_ok_add_None; eauto.
 Admitted.
 
+Theorem c_exp_correct: forall e,
+  goal_exp e.
+Proof.
+  induction e.
+  - eapply c_exp_Var.
+  - eapply c_exp_Const.
+  - eapply c_exp_Add; eauto.
+  - eapply c_exp_Sub; eauto.
+  - eapply c_exp_Div; eauto.
+  - eapply c_exp_Read; eauto.
+Qed.
 
+Ltac eval_exp_correct_tac :=
+  lazymatch reverse goal with
+  | [
+    Heval: eval_exp _ _ = (?res, _) |- _
+  ] =>
+    let Hneq := fresh "H" in
+    assert (res <> Stop Crash) as Hneq by congruence;
+    eapply c_exp_correct in Heval; eauto;
+    eapply Heval in Hneq; eauto; clear Heval; eauto; cleanup
+  end.
 
+Ltac eval_test_goal_tac :=
+  lazymatch reverse goal with
+  | [
+    Hgoal: goal_test ?tst,
+    Heval: eval_test ?tst _ = (?res, _) |- _
+  ] =>
+    unfold goal_test in Hgoal;
+    eapply Hgoal in Heval; eauto; clear Hgoal; cleanup
+  end.
 
+Ltac steps_inst_tac :=
+  lazymatch goal with
+  | [ H: steps _ _ |- _ ] =>
+    rw ltac:(specialize (steps_instructions _ _ _ _ H))
+  end.
+
+Ltac inst_has_stack c :=
+  match reverse goal with
+  | [ H: has_stack _ _ |- _ ] =>
+    instantiate(1 := c) in H
+  end.
+
+Ltac has_stack_even_tac :=
+  match goal with
+  | [ H: has_stack _ _ |- _ ] =>
+    specialize (has_stack_even _ _ H) as ?;
+    unfold has_stack in H
+  end.
+
+Ltac mem_inv_pmap_subsume_tac p p1 :=
+  lazymatch goal with
+  | [
+    Hmem: mem_inv p _ _,
+    Hsub1: pmap_subsume p p1 |- _
+  ] =>
+    eapply mem_inv_pmap_subsume
+      with (pmap1 := p1) (pmap := p) in Hmem; eauto
+  | [
+    Hmem: mem_inv p _ _,
+    Hsub1: pmap_subsume p ?x,
+    Hsub2: pmap_subsume ?x p1 |- _
+  ] =>
+    eapply pmap_subsume_trans with (pmap3 := p1) in Hsub1; eauto;
+    eapply mem_inv_pmap_subsume
+      with (pmap1 := p1) (pmap := p) in Hmem; eauto
+  end.
+
+Ltac env_ok_pmap_subsume_tac p p1 :=
+  lazymatch goal with
+  | [
+    Hmem: env_ok _ _ _ p _ _,
+    Hsub1: pmap_subsume p p1 |- _
+  ] =>
+    eapply env_ok_pmap_subsume
+      with (pmap1 := p1) (pmap := p) in Hmem; eauto
+  | [
+    Hmem: env_ok _ _ _ p _ _,
+    Hsub1: pmap_subsume p ?x,
+    Hsub2: pmap_subsume ?x p1 |- _
+  ] =>
+    eapply pmap_subsume_trans with (pmap3 := p1) in Hsub1; eauto;
+    eapply env_ok_pmap_subsume
+      with (pmap1 := p1) (pmap := p) in Hmem; eauto
+  end.
+
+Theorem c_test_Test_Less: forall (cm : cmp) (e1 e2 : exp),
+  cm = ImpSyntax.Less ->
+  goal_test (Test cm e1 e2).
+Proof.
+  intros.
+  unfold goal_test; intros.
+  simpl eval_test in *.
+  simpl c_exp in *; unfold c_test_jump in *; unfold dlet in *.
+  unfold bind in *.
+  destruct (eval_exp e1 s) eqn:?; simpl in *.
+  destruct o eqn:?; subst.
+  2: eval_exp_contr_stop_tac.
+  destruct (eval_exp e2 s0) eqn:?; simpl in *.
+  destruct o eqn:?; subst.
+  2: eval_exp_contr_stop_tac.
+  unfold eval_cmp in *.
+  destruct v eqn:?; unfold_outcome; cleanup; subst.
+  destruct v0 eqn:?; unfold_outcome; cleanup; subst.
+  destruct (c_exp e1 (pc t) vs) eqn:?; simpl in *.
+  destruct (c_exp e2 n (None :: vs)) eqn:?; simpl in *.
+  specialize (eval_exp_pure e1 _ _ _ Heqp).
+  specialize (eval_exp_pure e2 _ _ _ Heqp0).
+  intros; subst.
+  repeat rewrite code_in_append in *; cleanup.
+  eval_exp_correct_tac.
+  rwr ltac:(specialize (c_exp_length e1 _ _ _ _ Heqp1)).
+  specialize (c_exp_length e2 _ _ _ _ Heqp2) as ?; subst.
+  destruct x; destruct s; cleanup; subst.
+  2: eexists; eexists; split; eauto.
+  unfold exp_res_rel in *; cleanup; subst.
+  steps_inst_tac.
+  eval_exp_correct_tac.
+  1: destruct x1; destruct s0; cleanup; subst.
+  2: repeat eexists; repeat split; [eapply steps_trans|..]; eauto; simpl; eauto.
+  2: eapply pmap_subsume_trans; eauto.
+  all: unfold exp_res_rel in *; cleanup.
+  all: try rewrite <- H24 in *.
+  all: unfold state_rel in *; cleanup.
+  1: inst_has_stack (Word x :: curr).
+  1: {
+    repeat has_stack_even_tac; cleanup.
+    unfold env_ok in *; cleanup.
+    steps_inst_tac.
+    mem_inv_pmap_subsume_tac pmap x2.
+    rewrite <- H22 in *.
+    simpl in *.
+    cleanup; subst.
+    destruct ((Naive.unsigned w) <? (Naive.unsigned w0))%Z eqn:?.
+    1: {
+      eexists; eexists.
+      split.
+      1: {
+        eapply steps_trans.
+        1: eauto.
+        eapply steps_trans.
+        1: eauto.
+        eapply steps_trans.
+        1: eapply steps_step_same.
+        1: eapply step_mov; eauto.
+        eapply steps_trans.
+        1: eapply steps_step_same.
+        1: eapply step_pop; eauto.
+        eapply steps_trans.
+        1: eapply steps_step_same.
+        1: eapply step_pop; eauto.
+        eapply steps_trans.
+        1: eapply steps_step_same.
+        1: eapply step_jump; eauto.
+        1: econstructor; simpl; eauto.
+        eapply steps_refl.
+      }
+      simpl.
+      unfold code_rel in *; cleanup; eauto.
+      try rewrite Heqb.
+      bin_exp_post_tac.
+    }
+    eexists; eexists.
+    split.
+    1: {
+      eapply steps_trans.
+      1: eauto.
+      eapply steps_trans.
+      1: eauto.
+      eapply steps_trans.
+      1: eapply steps_step_same.
+      1: eapply step_mov; eauto.
+      eapply steps_trans.
+      1: eapply steps_step_same.
+      1: eapply step_pop; eauto.
+      eapply steps_trans.
+      1: eapply steps_step_same.
+      1: eapply step_pop; eauto.
+      eapply steps_trans.
+      1: eapply steps_step_same.
+      1: eapply step_jump; eauto.
+      1: econstructor; simpl; eauto.
+      eapply steps_trans.
+      1: eapply steps_step_same.
+      1: eapply step_jump; eauto.
+      1: simpl; rewrite Heqb; eauto.
+      1: econstructor; simpl; eauto.
+      eapply steps_refl.
+    }
+    simpl.
+    unfold code_rel in *; cleanup; eauto.
+    try rewrite Heqb.
+    bin_exp_post_tac.
+  }
+  all: eauto.
+  unfold state_rel in *; cleanup.
+  eapply env_ok_add_None; eauto.
+Qed.
+
+Theorem c_test_Test_Equal: forall (cm : cmp) (e1 e2 : exp),
+  cm = ImpSyntax.Equal ->
+  goal_test (Test cm e1 e2).
+Proof.
+  intros.
+  unfold goal_test; intros.
+  simpl eval_test in *.
+  simpl c_exp in *; unfold c_test_jump in *; unfold dlet in *.
+  unfold bind in *.
+  destruct (eval_exp e1 s) eqn:?; simpl in *.
+  destruct o eqn:?; subst.
+  2: eval_exp_contr_stop_tac.
+  destruct (eval_exp e2 s0) eqn:?; simpl in *.
+  destruct o eqn:?; subst.
+  2: eval_exp_contr_stop_tac.
+  unfold eval_cmp in *.
+  destruct v eqn:?; unfold_outcome; cleanup; subst.
+  destruct v0 eqn:?; unfold_outcome; cleanup; subst.
+  destruct (c_exp e1 (pc t) vs) eqn:?; simpl in *.
+  destruct (c_exp e2 n (None :: vs)) eqn:?; simpl in *.
+  specialize (eval_exp_pure e1 _ _ _ Heqp).
+  specialize (eval_exp_pure e2 _ _ _ Heqp0).
+  intros; subst.
+  repeat rewrite code_in_append in *; cleanup.
+  eval_exp_correct_tac.
+  rwr ltac:(specialize (c_exp_length e1 _ _ _ _ Heqp1)).
+  specialize (c_exp_length e2 _ _ _ _ Heqp2) as ?; subst.
+  destruct x; destruct s; cleanup; subst.
+  2: eexists; eexists; split; eauto.
+  unfold exp_res_rel in *; cleanup; subst.
+  try steps_inst_tac.
+  eval_exp_correct_tac.
+  1: destruct x1; destruct s0; cleanup; subst.
+  2: repeat eexists; repeat split; [eapply steps_trans|..]; eauto; simpl; eauto.
+  2: eapply pmap_subsume_trans; eauto.
+  all: unfold exp_res_rel in *; cleanup.
+  all: try rewrite <- H24 in *.
+  all: unfold state_rel in *; cleanup.
+  1: inst_has_stack (Word x :: curr).
+  1: {
+    repeat has_stack_even_tac; cleanup.
+    unfold env_ok in *; cleanup.
+    steps_inst_tac.
+    mem_inv_pmap_subsume_tac pmap x2.
+    rewrite <- H22 in *.
+    simpl in *.
+    cleanup; subst.
+    destruct ((Naive.unsigned w) =? (Naive.unsigned w0))%Z eqn:?.
+    1: {
+      eexists; eexists.
+      split.
+      1: {
+        eapply steps_trans.
+        1: eauto.
+        eapply steps_trans.
+        1: eauto.
+        eapply steps_trans.
+        1: eapply steps_step_same.
+        1: eapply step_mov; eauto.
+        eapply steps_trans.
+        1: eapply steps_step_same.
+        1: eapply step_pop; eauto.
+        eapply steps_trans.
+        1: eapply steps_step_same.
+        1: eapply step_pop; eauto.
+        eapply steps_trans.
+        1: eapply steps_step_same.
+        1: eapply step_jump; eauto.
+        1: econstructor; simpl; eauto.
+        eapply steps_refl.
+      }
+      simpl.
+      unfold code_rel in *; cleanup; eauto.
+      try rewrite Heqb.
+      bin_exp_post_tac.
+    }
+    eexists; eexists.
+    split.
+    1: {
+      eapply steps_trans.
+      1: eauto.
+      eapply steps_trans.
+      1: eauto.
+      eapply steps_trans.
+      1: eapply steps_step_same.
+      1: eapply step_mov; eauto.
+      eapply steps_trans.
+      1: eapply steps_step_same.
+      1: eapply step_pop; eauto.
+      eapply steps_trans.
+      1: eapply steps_step_same.
+      1: eapply step_pop; eauto.
+      eapply steps_trans.
+      1: eapply steps_step_same.
+      1: eapply step_jump; eauto.
+      1: econstructor; simpl; eauto.
+      eapply steps_trans.
+      1: eapply steps_step_same.
+      1: eapply step_jump; eauto.
+      1: simpl; rewrite Heqb; eauto.
+      1: econstructor; simpl; eauto.
+      eapply steps_refl.
+    }
+    simpl.
+    unfold code_rel in *; cleanup; eauto.
+    try rewrite Heqb.
+    bin_exp_post_tac.
+  }
+  all: eauto.
+  unfold state_rel in *; cleanup.
+  eapply env_ok_add_None; eauto.
+Qed.
+
+Theorem c_test_Test: forall (cm : cmp) (e1 e2 : exp),
+  goal_test (Test cm e1 e2).
+Proof.
+  destruct cm; intros.
+  - eapply c_test_Test_Less; reflexivity.
+  - eapply c_test_Test_Equal; reflexivity.
+Qed.
+
+Theorem c_test_And: ∀ (tst1 tst2 : test),
+  goal_test tst1 -> goal_test tst2 ->
+  goal_test (ImpSyntax.And tst1 tst2).
+Proof.
+  intros.
+  unfold goal_test; intros.
+  simpl eval_test in *.
+  simpl c_test_jump in *; unfold dlet in *.
+  unfold bind in *.
+  destruct (eval_test tst1 s) eqn:?; simpl in *.
+  destruct o eqn:?; subst; cleanup.
+  destruct (eval_test tst2 s0) eqn:?; simpl in *.
+  destruct o eqn:?; subst; cleanup.
+  unfold_outcome; cleanup.
+  destruct (c_test_jump tst1) eqn:?; simpl in *.
+  destruct (c_test_jump tst2) eqn:?; simpl in *.
+  specialize (eval_test_pure tst1 _ _ _ Heqp).
+  specialize (eval_test_pure tst2 _ _ _ Heqp0).
+  intros; subst.
+  repeat rewrite code_in_append in *; cleanup.
+  assert (pc t + 1 + 1 = pc t + 2) as Htmp; [lia|]; rewrite Htmp in *; clear Htmp.
+  rwr ltac:(specialize (c_test_length tst1 _ _ _ _ _ _ Heqp1)).
+  assert (pc t + 2 = pc (set_pc (if true then pc t + 2 else pc t + 1) t)) as Htmp by (simpl; reflexivity).
+  rewrite Htmp in *; clear Htmp.
+  eval_test_goal_tac.
+  destruct x; destruct s; cleanup; subst.
+  2: {
+    eexists; eexists; split.
+    1: {
+      eapply steps_trans.
+      1: eapply steps_step_same.
+      1: eapply step_jump.
+      1: simpl; eauto.
+      1: constructor.
+      eauto.
+    }
+    split; eauto.
+  }
+  assert (n = pc (set_pc n s)) as Htmp by (simpl; reflexivity); rewrite Htmp in *; clear Htmp.
+  unfold goal_test in H0; eapply H0 in Heqp0; clear H0; cleanup.
+  4: eauto.
+  8: exact H11.
+  all: eauto.
+  1: destruct x; destruct s0; cleanup; subst.
+  2: {
+    destruct v eqn:?.
+    all: mem_inv_pmap_subsume_tac pmap x0.
+    all: rewrite <- H16 in *.
+    all: specialize (steps_instructions _ _ _ _ H) as Htmp; simpl in Htmp; rewrite Htmp in H9; clear Htmp.
+    1: {
+      eexists; eexists; split.
+      1: {
+        eapply steps_trans.
+        1: eapply steps_step_same.
+        1: eapply step_jump.
+        1: simpl; eauto.
+        1: constructor.
+        eapply steps_trans.
+        1: eauto.
+        eapply steps_trans.
+        1: eapply steps_step_same.
+        1: eapply step_jump.
+        1: simpl; eauto.
+        1: constructor.
+        simpl; eauto.
+      }
+      split; eauto.
+      split; [eapply pmap_subsume_trans|]; eauto.
+    }
+    eexists; eexists; split.
+    1: {
+      eapply steps_trans.
+      1: eapply steps_step_same.
+      1: eapply step_jump.
+      1: simpl; eauto.
+      1: constructor.
+      eauto.
+    }
+    simpl.
+    split; [exact H11|]; eauto.
+  }
+  3: simpl in *; unfold state_rel in *; cleanup; rwr ltac:(specialize (steps_instructions _ _ _ _ H)); eauto.
+  2: rewrite memory_set_memory; eapply env_ok_pmap_subsume; eauto.
+  all: unfold state_rel in *; cleanup.
+  destruct v eqn:?; subst.
+  1: {
+    destruct v0 eqn:?; subst.
+    - eexists; eexists; split. (* true && true *)
+      all: rewrite <- H16 in *.
+      all: specialize (steps_instructions _ _ _ _ H) as Htmp; simpl in Htmp; rewrite Htmp in H9; clear Htmp.
+      1: {
+        eapply steps_trans.
+        1: eapply steps_step_same.
+        1: eapply step_jump.
+        1: simpl; eauto.
+        1: constructor.
+        eapply steps_trans.
+        1: eauto.
+        eapply steps_trans.
+        1: eapply steps_step_same.
+        1: eapply step_jump.
+        1: simpl; eauto.
+        1: constructor.
+        simpl; eauto.
+      }
+      simpl.
+      unfold code_rel in *; cleanup; eauto.
+      bin_exp_post_tac.
+    - eexists; eexists; split. (* true && false *)
+      all: rewrite <- H16 in *.
+      all: specialize (steps_instructions _ _ _ _ H) as Htmp; simpl in Htmp; rewrite Htmp in H9; clear Htmp.
+      1: {
+        eapply steps_trans.
+        1: eapply steps_step_same.
+        1: eapply step_jump.
+        1: simpl; eauto.
+        1: constructor.
+        eapply steps_trans.
+        1: eauto.
+        eapply steps_trans.
+        1: eapply steps_step_same.
+        1: eapply step_jump.
+        1: simpl; eauto.
+        1: constructor.
+        simpl; eauto.
+      }
+      simpl.
+      unfold code_rel in *; cleanup; eauto.
+      bin_exp_post_tac.
+  }
+  eexists; eexists; split. (* false && _ *)
+  all: specialize (steps_instructions _ _ _ _ H) as Htmp; simpl in Htmp; rewrite Htmp in H9; clear Htmp.
+  1: {
+    eapply steps_trans.
+    1: eapply steps_step_same.
+    1: eapply step_jump.
+    1: simpl; eauto.
+    1: constructor.
+    eauto.
+  }
+  simpl.
+  repeat split; eauto.
+  all: unfold code_rel in *; cleanup; eauto.
+  2: eexists; eexists; eauto.
+  1: try eapply pmap_subsume_trans; eauto.
+  mem_inv_pmap_subsume_tac x0 x1.
+Qed.
+
+Theorem c_test_Or: ∀ (tst1 tst2 : test),
+  goal_test tst1 -> goal_test tst2 ->
+  goal_test (ImpSyntax.Or tst1 tst2).
+Proof.
+  intros.
+  unfold goal_test; intros.
+  simpl eval_test in *.
+  simpl c_test_jump in *; unfold dlet in *.
+  unfold bind in *.
+  destruct (eval_test tst1 s) eqn:?; simpl in *.
+  destruct o eqn:?; subst; cleanup.
+  destruct (eval_test tst2 s0) eqn:?; simpl in *.
+  destruct o eqn:?; subst; cleanup.
+  unfold_outcome; cleanup.
+  destruct (c_test_jump tst1) eqn:?; simpl in *.
+  destruct (c_test_jump tst2) eqn:?; simpl in *.
+  specialize (eval_test_pure tst1 _ _ _ Heqp).
+  specialize (eval_test_pure tst2 _ _ _ Heqp0).
+  intros; subst.
+  repeat rewrite code_in_append in *; cleanup.
+  assert (pc t + 1 + 1 = pc t + 2) as Htmp; [lia|]; rewrite Htmp in *; clear Htmp.
+  rwr ltac:(specialize (c_test_length tst1 _ _ _ _ _ _ Heqp1)).
+  assert (pc t + 2 = pc (set_pc (if true then pc t + 2 else pc t + 1) t)) as Htmp by (simpl; reflexivity).
+  rewrite Htmp in *; clear Htmp.
+  eval_test_goal_tac.
+  destruct x; destruct s; cleanup; subst.
+  2: {
+    eexists; eexists; split.
+    1: {
+      eapply steps_trans.
+      1: eapply steps_step_same.
+      1: eapply step_jump.
+      1: simpl; eauto.
+      1: constructor.
+      eauto.
+    }
+    split; eauto.
+  }
+  assert (n = pc (set_pc n s)) as Htmp by (simpl; reflexivity); rewrite Htmp in *; clear Htmp.
+  unfold goal_test in H0; eapply H0 in Heqp0; clear H0; cleanup.
+  4: eauto.
+  8: exact H11.
+  all: eauto.
+  1: destruct x; destruct s0; cleanup; subst.
+  2: {
+    destruct v eqn:?.
+    all: mem_inv_pmap_subsume_tac pmap x0.
+    all: rewrite <- H16 in *.
+    all: specialize (steps_instructions _ _ _ _ H) as Htmp; simpl in Htmp; rewrite Htmp in H9; clear Htmp.
+    1: {
+      eexists; eexists; split.
+      1: {
+        eapply steps_trans.
+        1: eapply steps_step_same.
+        1: eapply step_jump.
+        1: simpl; eauto.
+        1: constructor.
+        eauto.
+      }
+      simpl.
+      split; [exact H11|]; eauto.
+    }
+    eexists; eexists; split.
+    1: {
+      eapply steps_trans.
+      1: eapply steps_step_same.
+      1: eapply step_jump.
+      1: simpl; eauto.
+      1: constructor.
+      eapply steps_trans.
+      1: eauto.
+      eapply steps_trans.
+      1: eapply steps_step_same.
+      1: eapply step_jump.
+      1: simpl; eauto.
+      1: constructor.
+      simpl; eauto.
+    }
+    split; eauto.
+    split; [eapply pmap_subsume_trans|]; eauto.
+  }
+  3: simpl in *; unfold state_rel in *; cleanup; rwr ltac:(specialize (steps_instructions _ _ _ _ H)); eauto.
+  2: rewrite memory_set_memory; eapply env_ok_pmap_subsume; eauto.
+  all: unfold state_rel in *; cleanup.
+  destruct v eqn:?; subst.
+  1: { (* true || _ *)
+    eexists; eexists; split.
+    all: specialize (steps_instructions _ _ _ _ H) as Htmp; simpl in Htmp; rewrite Htmp in H9; clear Htmp.
+    1: {
+      eapply steps_trans.
+      1: eapply steps_step_same.
+      1: eapply step_jump.
+      1: simpl; eauto.
+      1: constructor.
+      eauto.
+    }
+    simpl.
+    repeat split; eauto.
+    all: unfold code_rel in *; cleanup; eauto.
+    2: eexists; eexists; eauto.
+    1: try eapply pmap_subsume_trans; eauto.
+    mem_inv_pmap_subsume_tac x0 x1.
+  }
+  destruct v0 eqn:?; subst.
+  - eexists; eexists; split. (* false || true *)
+    all: rewrite <- H16 in *.
+    all: specialize (steps_instructions _ _ _ _ H) as Htmp; simpl in Htmp; rewrite Htmp in H9; clear Htmp.
+    1: {
+      eapply steps_trans.
+      1: eapply steps_step_same.
+      1: eapply step_jump.
+      1: simpl; eauto.
+      1: constructor.
+      eapply steps_trans.
+      1: eauto.
+      eapply steps_trans.
+      1: eapply steps_step_same.
+      1: eapply step_jump.
+      1: simpl; eauto.
+      1: constructor.
+      simpl; eauto.
+    }
+    simpl.
+    unfold code_rel in *; cleanup; eauto.
+    bin_exp_post_tac.
+  - eexists; eexists; split. (* false || false *)
+    all: rewrite <- H16 in *.
+    all: specialize (steps_instructions _ _ _ _ H) as Htmp; simpl in Htmp; rewrite Htmp in H9; clear Htmp.
+    1: {
+      eapply steps_trans.
+      1: eapply steps_step_same.
+      1: eapply step_jump.
+      1: simpl; eauto.
+      1: constructor.
+      eapply steps_trans.
+      1: eauto.
+      eapply steps_trans.
+      1: eapply steps_step_same.
+      1: eapply step_jump.
+      1: simpl; eauto.
+      1: constructor.
+      simpl; eauto.
+    }
+    simpl.
+    unfold code_rel in *; cleanup; eauto.
+    bin_exp_post_tac.
+Qed.
+
+Theorem c_test_Not: ∀ (tst : test),
+  goal_test tst ->
+  goal_test (ImpSyntax.Not tst).
+Proof.
+  intros.
+  unfold goal_test; intros.
+  simpl eval_test in *.
+  simpl c_test_jump in *; unfold dlet in *.
+  unfold bind in *.
+  destruct (eval_test tst s) eqn:?; simpl in *.
+  destruct o eqn:?; subst; cleanup.
+  unfold_outcome; cleanup.
+  destruct (c_test_jump tst) eqn:?; simpl in *.
+  specialize (eval_test_pure tst _ _ _ Heqp).
+  intros; subst.
+  repeat rewrite code_in_append in *; cleanup.
+  eval_test_goal_tac.
+  destruct x eqn:?; destruct s eqn:?; cleanup.
+  2: eexists; eexists; split; eauto.
+  destruct v eqn:?; subst.
+  1: {
+    eexists; eexists; split.
+    1: eauto.
+    simpl.
+    split; eauto.
+  }
+  eexists; eexists; split.
+  1: eauto.
+  simpl.
+  split; eauto.
+Qed.
+
+Theorem c_test_correct: forall (tst: test),
+  goal_test tst.
+Proof.
+  induction tst.
+  - eapply c_test_Test.
+  - eapply c_test_And; eauto.
+  - eapply c_test_Or; eauto.
+  - eapply c_test_Not; eauto.
+Qed.
